segmento de suma maxima siguiendo la metodologia

ejemplos/calculo_de_programas/segmento_de_suma_maxima.dfy
@@ -4,36 +4,73 @@ function suma(p:nat, q:nat, A: seq<int>): int
     if q <= p then 0 else suma(p, q-1, A) + A[q-1]
 }
 
-method segmento_de_suma_maxima(A: seq<int>) returns (r: int, p: nat, q: nat)
-    ensures 0 <= p <= q <= |A|
-    ensures r == suma(p, q, A)
-    ensures forall i, j :: 0 <= i <= j <= |A| ==> suma(i, j, A) <= r
+predicate es_suma_maxima(A: seq<int>, r: int) {
+    (exists p, q :: 0 <= p <= q <= |A| && suma(p, q, A) == r) &&
+    (forall i, j :: 0 <= i <= j <= |A| ==> suma(i, j, A) <= r)
+}
+
+method test_suma()
 {
-    var n, u := 0, 0;
-    var u_p := 0;
-    p, q := 0, 0;
+    assert suma(0, 3, [1,2,-3,4,5]) == 0;
+    assert suma(0, 4, [1,2,-3,4,5]) == 4;
+    assert suma(3, 5, [1,2,-3,4,5]) == 9;
+    assert suma(4, 4, [1,2,-3,4,5]) == 0;
+}
+
+method test_es_suma_maxima(){
+    assert es_suma_maxima([1,2,-3], 3);
+    assert suma(0, 3, [1,2,3]) == 6;
+    assert es_suma_maxima([1,2,3], 6);
+}
+
+predicate invariante(k: int, A: seq<int>, r: int, u: int){
+    0 <= k <= |A| &&
+    (exists p_u :: 0 <= p_u <= k && suma(p_u, k, A) == u) &&
+    (forall i :: 0 <= i <= k ==> suma(i, k, A) <= u) &&
+    (exists p, q :: 0 <= p <= q <= k && suma(p, q, A) == r) &&
+    (forall i, j :: 0 <= i <= j <= k ==> suma(i, j, A) <= r)
+}
+
+method inicializacion(A: seq<int>) returns (k: int, r: int, u: int)
+    ensures invariante(k, A, r, u)
+{
+    k := 0;
     r := 0;
-    while n < |A|
-        decreases |A| - n
-        invariant 0 <= n <= |A|
-        invariant 0 <= u_p <= n
-        invariant u == suma(u_p, n, A)
-        invariant forall i :: 0 <= i <= n ==> suma(i, n, A) <= u
-        invariant 0 <= p <= q <= |A|
-        invariant r == suma(p, q, A)
-        invariant forall i, j :: 0 <= i <= j <= n ==> suma(i, j, A) <= r
+    u := 0;
+    assert suma(0, 0, A) == 0;
+}
+
+method cuerpo(k: int, A: seq<int>, r: int, u:int) returns (k': int, r': int, u': int)
+    requires k < |A|
+    requires invariante(k, A, r, u)
+    ensures invariante(k', A, r', u')
+    ensures k' > k
+{
+    if u + A[k] < 0 {
+        u' := 0;
+        assert suma(k+1, k+1, A) == u';
+    } else {
+        u' := u + A[k];
+        ghost var p_u :| (0 <= p_u <= k && suma(p_u, k, A) == u) && (forall i :: 0 <= i <= k ==> suma(i, k, A) <= u);
+        assert suma(p_u, k+1, A) == u';
+    }
+    if u' > r {
+        r' := u';
+    } else {
+        r' := r;
+    }
+    k' := k + 1;
+}
+
+method segmento_de_suma_maxima(A: seq<int>) returns (r: int)
+    ensures es_suma_maxima(A, r)
+{
+    var k: int, u: int;
+    k, r, u := inicializacion(A);
+    while (k < |A|)
+        decreases |A| - k
+        invariant invariante(k, A, r, u)
     {
-        if u + A[n] > r {
-            r := u + A[n];
-            p := u_p;
-            q := n + 1;
-        }
-        if u + A[n] > 0 {
-            u := u + A[n];
-        } else {
-            u_p := n + 1;
-            u := 0;
-        }
-        n := n + 1;
+        k, r, u := cuerpo(k, A, r, u);
     }
 }
