ejemplos/calculo_de_programas/segmento_de_suma_maxima_con_indices.dfy
@@ -1,0 +1,47 @@
+function suma(p:nat, q:nat, A: seq<int>): int
+    requires 0 <= p <= q <= |A|
+{
+    if q <= p then 0 else suma(p, q-1, A) + A[q-1]
+}
+
+method test_suma()
+{
+    assert suma(0, 3, [1,2,3,4,5]) == 6;
+    assert suma(0, 4, [1,2,3,4,5]) == 10;
+    assert suma(2, 4, [1,2,3,4,5]) == 7;
+    assert suma(4, 4, [1,2,3,4,5]) == 0;
+}
+
+method segmento_de_suma_maxima(A: seq<int>) returns (r: int, p: nat, q: nat)
+    ensures 0 <= p <= q <= |A|
+    ensures r == suma(p, q, A)
+    ensures forall i, j :: 0 <= i <= j <= |A| ==> suma(i, j, A) <= r
+{
+    var n, u := 0, 0;
+    var u_p := 0;
+    p, q := 0, 0;
+    r := 0;
+    while n < |A|
+        decreases |A| - n
+        invariant 0 <= n <= |A|
+        invariant 0 <= u_p <= n
+        invariant u == suma(u_p, n, A)
+        invariant forall i :: 0 <= i <= n ==> suma(i, n, A) <= u
+        invariant 0 <= p <= q <= |A|
+        invariant r == suma(p, q, A)
+        invariant forall i, j :: 0 <= i <= j <= n ==> suma(i, j, A) <= r
+    {
+        if u + A[n] > r {
+            r := u + A[n];
+            p := u_p;
+            q := n + 1;
+        }
+        if u + A[n] > 0 {
+            u := u + A[n];
+        } else {
+            u_p := n + 1;
+            u := 0;
+        }
+        n := n + 1;
+    }
+}
